generational/spec/GC.Gen.MinorCollectForwarding.fsti
@@ -85,7 +85,6 @@ val combined_reachable_minor_has_fwd
   (minor: minor_state) (major: heap) (fp: U64.t) (roots: seq U64.t)
   : Lemma
     (requires
-      RBridge.major_field_one_plus_in_remembered minor major /\
       RBridge.major_field_zero_no_minor minor major /\
       RBridge.remembered_roots_in_roots major roots /\
       well_formed_heap major /\
@@ -129,7 +128,6 @@ val combined_reachable_images_valid_or_infix
   : Lemma
     (requires
       GenInv.collection_heap_shape minor major fp /\
-      RBridge.major_field_one_plus_in_remembered minor major /\
       RBridge.major_field_zero_no_minor minor major /\
       RBridge.remembered_roots_in_roots major roots /\
       CheneyBFS.cheney_no_oom minor major fp roots)
@@ -162,8 +160,7 @@ let minor_collect_full_forwarding_kernel
     // Normal images are injective and non-blue.
     CheneyPres.fwd_normal_injective fwd prom.major_final /\
     CheneyPres.fwd_targets_not_blue fwd prom.major_final /\
-    (RBridge.major_field_one_plus_in_remembered minor major /\
-     RBridge.major_field_zero_no_minor minor major /\
+    (RBridge.major_field_zero_no_minor minor major /\
      RBridge.remembered_roots_in_roots major roots ==>
      combined_reachable_images_valid_or_infix_prop minor major fp roots))
 
